EvmCompiler/Functions.lean
@@ -4,4 +4,6 @@ import EvmCompiler.Functions.Compiler
 import EvmCompiler.Functions.SourceSemantics
 import EvmCompiler.Functions.EffectSemantics
 import EvmCompiler.Functions.InteractionSemantics
+import EvmCompiler.Functions.AllocationInteractionRelation
+import EvmCompiler.Functions.AllocationInteractionExpression
 import EvmCompiler.Functions.Semantics
